\documentclass{article}
\usepackage[colorlinks]{hyperref}
\usepackage[hmargin=1in,vmargin=1in]{geometry}
\usepackage{amsmath,cancel,color,mathrsfs}
\newcommand{\mycan}[2]{{\textcolor{red}{\cancelto{#2}{\textcolor{blue}
{#1}}}}}
\begin{document}
\hfill Tanzim Amin

\hfill Exam 3 Take Home
\\
Derivation of $\mathscr{L} \{ t \} $:
\begin{align*}
\mathscr{L} \{ t \} &= \displaystyle{\int_0^{\infty}
t e^{-st} \, dt}\\
&=\lim_{b \rightarrow \infty}  \dfrac{-t}{s}e^{-st} - \dfrac{1}{s^2}e^{-st}\bigg|_0^{b}\\ 
\newline\\
&=\lim_{b \rightarrow \infty} \, \left[\left(\mycan{\dfrac{-b}{s}e^{-sb}}{0} - \mycan{\dfrac{1}{s^2}e^{-sb}}{0}\right) - \left(\mycan{\dfrac{-0}{s}e^{-s(0)}}{0}- \dfrac{1}{s^2}e^{-s(0)}\right)\right]\\
\newline\\
&= 0 - \left(0 - \dfrac{1}{s^2}\right)\\
\newline\\
&= \dfrac{1}{s^2}, \quad  s > 0\\
\end{align*}
\textmd{Derivation of $\mathscr{L} \{ \cos(kt) \} $}:
\end{center}
\begin{center}$\mathscr{L} \{ \cos(kt) \} &= \displaystyle{\int_0^{\infty}e^{-st}\cos(kt) \, dt}\\\end{center}
&= \lim\limits_{N \to \infty}
\displaystyle{\int_0^{N}e^{-st}\cos(kt)dt}\\ 
\newline\\
\int e^{-st}\cos(kt) \, dt  {\color{green} + \int\dfrac{s^2}{k^2}e^{-st}\cos(kt) \, dt} = \dfrac{e^{-st}}{k}\sin(kt) \ - \dfrac{se^{-st}}{k^2}\cos(kt)-\int\dfrac{s^2}{k^2}e^{-st}\cos(kt) \, dt 
{\color{green} + \int\dfrac{s^2}{k^2}e^{-st}\cos(kt) \, dt} \\ \newline\\
\dfrac{k^2+s^2}{k^2}\int e^{-st}\cos(kt) \, dt = \dfrac{e^{-st}}{k}\sin(kt) - \dfrac{se^{-st}}{k^2}\cos(kt)\\
\newline\\
&= \dfrac{k^2}{s^2+k^2}\left(\dfrac{e^{-st}}{k}\sin(kt)- \dfrac{se^{-st}}{k^2}\cos(kt)\right)\\ 
\newline\\
&=\lim_{N \rightarrow \infty}\left(\dfrac{k}{s^2+k^2}e^{-st}\sin(kt)-\dfrac{s}{s^2+k^2}e^{-st}\cos(kt)\right)\bigg|_0^{N}\\ 
\newline\\
&=\lim_{N \rightarrow \infty}\left(\mycan{\dfrac{k}{s^2+k^2}e^{-sN}\sin(kN)}{0}-\mycan{\dfrac{s}{s^2+k^2}e^{-sN}\cos(kN)}{0}\right) - \left(\mycan{\dfrac{k}{s^2+k^2}e^{-s(0)}\sin(k*0)}{0}- \dfrac{s}{s^2+k^2}e^{-s(0)}\cos(k*0)\right)\\
&= 0 - \left(0 - \dfrac{s}{s^2+k^2}\right)\\ 
\newline\\
&= \dfrac{s}{s^2+k^2}, \quad s>0




\end{align*}
\end{document}